hol/imp_compiler_progScript.sml
@@ -1,11 +1,752 @@
 Theory imp_compiler_prog
 Ancestors
-  arithmetic list pair finite_map string words
-  imp_compiler source_syntax
+  arithmetic list pair finite_map string
+  source_values source_syntax source_semantics
+  source_properties parsing codegen x64asm_syntax
+  words automation_lemmas printing parsing
+  imp_automation_lemmas
+  imp_compiler imp_to_asm imp_parsing
+Libs
+  mp_then wordsLib imp_automationLib
 
-(* Top-level IMP compiler:
-   source text  →  IMP AST  →  x64 assembly  →  assembly string *)
+val _ = temp_delsimps ["LT1_EQ0"]
+
+val _ = show_assums := true;
+
+(* codegen *)
+
+val res = to_deep APPEND;
+val res = to_deep codegenTheory.flatten_def;
+val res = to_deep (init_def |> SIMP_RULE std_ss []);
+val res = to_deep imp_to_asmTheory.lookup_def;
+val res = to_deep (LENGTH |> REWRITE_RULE [ADD1]);
+val res = to_deep imp_to_asmTheory.app_list_length_def;
+val res = to_deep imp_to_asmTheory.make_vs_from_binders_def;
+val res = to_deep imp_to_asmTheory.fltr_nms_def;
+val res = to_deep imp_to_asmTheory.rm_nms_def;
+val res = to_deep imp_to_asmTheory.call_v_stack_def;
+val res = to_deep imp_to_asmTheory.push_vs_def;
+val res = to_deep names_contain_def;
+val res = to_deep names_unique_def;
+val res = to_deep all_binders_def;
+val res = to_deep unique_binders_def;
+val res = to_deep imp_source_syntaxTheory.get_name_def;
+val res = to_deep imp_to_asmTheory.even_len_def;
+val res = to_deep imp_to_asmTheory.vs_bdrs_def;
+val res = to_deep imp_to_asmTheory.c_bdrs_def;
+val res = to_deep imp_to_asmTheory.c_pushes_def;
+val res = to_deep imp_to_asmTheory.c_read_def;
+val res = to_deep imp_to_asmTheory.c_write_def;
+val res = to_deep imp_to_asmTheory.index_of_def;
+
+Theorem num_case_rw[local]:
+  num_CASE x f g = if x = 0 then f else g (x - 1)
+Proof
+  Cases_on ‘x’ \\ fs []
+QED
+
+val res = to_deep (imp_to_asmTheory.c_assign_def |> SIMP_RULE std_ss [num_case_rw]);
+val res = to_deep (imp_to_asmTheory.c_alloc_def |> SRULE [AllocLoc_def]);
+val res = to_deep imp_to_asmTheory.make_ret_def;
+val res = to_deep imp_to_asmTheory.give_up_def;
+val res = to_deep imp_to_asmTheory.c_pops_def;
+val res = to_deep imp_to_asmTheory.c_call_def;
+val res = to_deep imp_to_asmTheory.c_cmp_def;
+val res = to_deep imp_to_asmTheory.c_store_def;
+val res = to_deep imp_to_asmTheory.c_var_def;
+val res = to_deep imp_to_asmTheory.c_const_def;
+val res = to_deep imp_to_asmTheory.c_add_def;
+val res = to_deep imp_to_asmTheory.c_sub_def;
+val res = to_deep imp_to_asmTheory.c_div_def;
+val res = to_deep imp_to_asmTheory.c_load_def;
+
+Theorem pairlet_imp:
+  ((let (a,b) = f in x a b) = case f of (a,b) => x a b) ∧
+  ((let (a,b,c) = g in y a b c) = case g of (a,b,c) => y a b c)
+Proof
+  Cases_on ‘f’ \\ simp []
+  \\ PairCases_on ‘g’ \\ simp []
+QED
+
+val res = to_deep (imp_to_asmTheory.c_exp_def |> SIMP_RULE std_ss [pairlet_imp]);
+
+val def = (imp_to_asmTheory.c_test_jump_def |> SIMP_RULE std_ss [pairlet_imp])
+val res = to_deep def; (* TODO *)
+
+Theorem c_test_jump_side:
+  c_test_jump_side t neg_label pos_label l vs
+Proof
+  cheat
+QED
+
+val _ = update_mem c_test_jump_side;
+
+val res = to_deep (imp_to_asmTheory.c_exps_def |> SIMP_RULE std_ss [pairlet_imp]);
+val res = to_deep abortLoc_def;
+val res = to_deep (imp_to_asmTheory.c_cmd_def |> SIMP_RULE std_ss [pairlet_imp]);
+
+Theorem c_cmd_side:
+  c_cmd_side c l fs vs
+Proof
+  cheat
+QED
+
+val _ = update_mem c_cmd_side;
+
+val res = to_deep (imp_to_asmTheory.c_fundef_def |> SIMP_RULE std_ss [pairlet_imp]);
+
+Definition mul256_def:
+  mul256 n =
+    let n = n + n in
+    let n = n + n in
+    let n = n + n in
+    let n = n + n in
+    let n = n + n in
+    let n = n + n in
+    let n = n + n in
+            n + n : num
+End
+
+val res = to_deep mul256_def;
+
+Theorem mul256_thm[simp]:
+  mul256_side n ∧
+  mul256 n = 256 * n
+Proof
+  fs [mul256_def,res]
+QED
+
+Definition name2str_def:
+  name2str n =
+    if n = 0 then "" else
+      let n_div = n DIV 256 in
+      let n_mul = mul256 n_div in
+      let k = n - n_mul in
+        if k < 42 then "" else
+        if 122 < k then "" else
+        if k = 46 then "" else
+        if n < 256 then STRING (CHR k) "" else
+          STRCAT (name2str n_div) (STRING (CHR k) "")
+End
+
+val res = to_deep name2str_def;
+
+Theorem N2ascii_eq_name2str:
+  ∀n. N2ascii n = name2str n
+Proof
+  ho_match_mp_tac name2str_ind \\ rw []
+  \\ once_rewrite_tac [name2str_def, N2ascii_def]
+  \\ IF_CASES_TAC >- gvs []
+  \\ simp_tac bool_ss [LET_THM]
+  \\ ‘n − mul256 (n DIV 256) = n MOD 256’ by
+   (‘0 < 256:num’ by simp []
+    \\ drule DIVISION
+    \\ disch_then $ qspec_then ‘n’ mp_tac
+    \\ strip_tac
+    \\ simp [])
+  \\ asm_rewrite_tac [] \\ fs []
+  \\ IF_CASES_TAC \\ simp []
+  \\ IF_CASES_TAC \\ simp []
+QED
+
+val res = to_deep (imp_to_asmTheory.c_fundefs_def
+                     |> SIMP_RULE std_ss [pairlet_imp,N2ascii_eq_name2str]);
+val res = to_deep imp_source_syntaxTheory.get_funcs_def;
+val res = to_deep (imp_to_asmTheory.codegen_def
+                     |> SIMP_RULE (srw_ss()) [pairlet_imp, name_def]);
+
+(* parser *)
+
+val h_code_def = define_code ‘
+  (defun h (x) (if (= (head x) '1) x (head (tail x))))’
+
+val t_code_def = define_code ‘
+  (defun t (x) (if (= (head x) '1) x (tail (tail x))))’
+
+val res = to_deep source_valuesTheory.el1_def;
+val res = to_deep source_valuesTheory.el2_def;
+val res = to_deep source_valuesTheory.el3_def;
+val res = to_deep imp_parsingTheory.v2list_def;
+val res = to_deep imp_parsingTheory.vs2args_def;
+val res = to_deep is_upper_def;
+val res = to_deep num2exp_def;
+
+Theorem num2exp_side[local]:
+  num2exp_side n
+Proof
+  simp [res]
+QED
+
+val _ = update_mem num2exp_side;
+
+val res = to_deep (imp_parsingTheory.v2exp_def |> SRULE [name_def]);
+val res = to_deep (v2cmp_def |> SRULE [name_def]);
+val res = to_deep (imp_parsingTheory.v2test_def |> SRULE [name_def]);
+val res = to_deep imp_parsingTheory.vs2exps_def;
+val res = to_deep (imp_parsingTheory.v2cmd_def |> SRULE [name_def]);
+val res = to_deep imp_parsingTheory.v2func_def;
+val res = to_deep imp_parsingTheory.v2funcs_def;
+val res = to_deep imp_parsingTheory.vs2prog_def;
+val res = to_deep (quote_def |> SIMP_RULE (srw_ss()) [name_def]);
+val res = to_deep (parse_def |> DefnBase.one_line_ify NONE |> Q.INST [‘v’|->‘input’]);
+val res = to_deep imp_parsingTheory.parser_def;
+
+(* lexer *)
+
+Definition mul256_def:
+  mul256 n =
+    let n = n + n in
+    let n = n + n in
+    let n = n + n in
+    let n = n + n in
+    let n = n + n in
+    let n = n + n in
+    let n = n + n in
+            n + n : num
+End
+
+val res = to_deep mul256_def;
+
+Theorem mul256_thm[simp]:
+  mul256_side n ∧
+  mul256 n = 256 * n
+Proof
+  fs [mul256_def,res]
+QED
+
+Definition mul10_def:
+  mul10 n =
+    let n2 = n + n in
+    let n4 = n2 + n2 in
+    let n5 = n4 + n in
+      n5 + n5 : num
+End
+
+val res = to_deep mul10_def;
+
+Theorem mul10_thm[simp]:
+  mul10_side n ∧
+  mul10 n = 10 * n
+Proof
+  fs [mul10_def,res]
+QED
+
+val read_num_code_def = define_code ‘
+  (defun read_num (acc next)
+     (if (< next '58)
+       (if (< next '48)
+         (cons acc next)
+         (read_num
+           (+ (mul10 acc) (- next '48))
+           (read)))
+       (cons acc next)))’
+
+val read_str_code_def = define_code ‘
+  (defun read_str (acc next)
+     (if (< next '123)
+       (if (< next '42)
+         (cons acc next)
+         (read_str
+           (+ (mul256 acc) next)
+           (read)))
+       (cons acc next)))’
+
+val read_any_code_def = define_code ‘
+  (defun read_any (next)
+     (if (< next '58)
+       (if (< next '48)
+         (read_str '0 next)
+         (read_num '0 next))
+       (read_str '0 next)))’
+
+Theorem read_num_thm:
+  ∀input s acc k rest.
+    read_num #"0" #"9" 10 (ORD #"0") acc input = (k, rest) ∧
+    lookup_fun (name "mul10") s.funs = SOME ([name "n"],mul10_code) ∧
+    lookup_fun (name "read_num") s.funs = SOME ([name "acc"; name "next"],read_num_code) ∧
+    s.input = fromList (TL input) ⇒
+    app (name "read_num") [Num acc; next (fromList input)] s
+      (Pair (Num k) (next (fromList rest)), s with input := fromList (TL rest))
+Proof
+  gen_tac \\ completeInduct_on ‘LENGTH input’
+  \\ rw [] \\ fs [PULL_FORALL]
+  \\ match_mp_tac (trans_app |> SIMP_RULE std_ss [LET_THM] |> MP_CANON |> GEN_ALL)
+  \\ fs [make_env_def]
+  \\ simp [read_num_code_def]
+  \\ simp [Eval_eq,PULL_EXISTS]
+  \\ fs [combinTheory.APPLY_UPDATE_THM,name_def]
+  \\ Cases_on ‘input’ \\ fs [next_def]
+  \\ fs [take_branch_def,return_def,Eval_eq,PULL_EXISTS,next_def,
+         combinTheory.APPLY_UPDATE_THM,eval_op_def,read_num_def]
+  \\ rpt BasicProvers.VAR_EQ_TAC
+  \\ fs [take_branch_def,return_def,Eval_eq,PULL_EXISTS,next_def,
+         combinTheory.APPLY_UPDATE_THM,eval_op_def,read_num_def]
+  THEN1 fs [state_component_equality]
+  \\ reverse IF_CASES_TAC
+  \\ fs [take_branch_def,return_def,Eval_eq,PULL_EXISTS,next_def,
+         combinTheory.APPLY_UPDATE_THM,eval_op_def,read_num_def]
+  THEN1 (rw [] \\ fs [state_component_equality,next_def])
+  \\ fs [take_branch_def,return_def,Eval_eq,PULL_EXISTS,next_def,
+         combinTheory.APPLY_UPDATE_THM,eval_op_def,read_num_def]
+  \\ IF_CASES_TAC
+  \\ fs [take_branch_def,return_def,Eval_eq,PULL_EXISTS,next_def,
+         combinTheory.APPLY_UPDATE_THM,eval_op_def,read_num_def]
+  THEN1 (rw [] \\ fs [state_component_equality,next_def])
+  \\ (theorem "mul10_app" |> DISCH_ALL |> Q.INST [‘n’|->‘acc’]
+         |> SIMP_RULE (srw_ss()) [] |> mp_tac)
+  \\ fs [name_def,llistTheory.LFINITE_fromList]
+  \\ strip_tac \\ goal_assum (first_assum o mp_then Any mp_tac)
+  \\ fs [] \\ Cases_on ‘t’ \\ fs [AND_IMP_INTRO]
+  \\ first_x_assum (first_assum o mp_then (Pos (el 2)) mp_tac)
+  \\ fs []
+  THEN1 (disch_then (qspec_then ‘s with input := fromList ""’ mp_tac) \\ fs [])
+  \\ disch_then (qspec_then ‘s with input := fromList t'’ mp_tac) \\ fs []
+QED
+
+Theorem read_str_thm:
+  ∀input s acc k rest.
+    read_num #"*" #"z" 256 0 acc input = (k, rest) ∧
+    lookup_fun (name "mul256") s.funs = SOME ([name "n"],mul256_code) ∧
+    lookup_fun (name "read_str") s.funs = SOME ([name "acc"; name "next"],read_str_code) ∧
+    s.input = fromList (TL input) ⇒
+    app (name "read_str") [Num acc; next (fromList input)] s
+      (Pair (Num k) (next (fromList rest)), s with input := fromList (TL rest))
+Proof
+  gen_tac \\ completeInduct_on ‘LENGTH input’
+  \\ rw [] \\ fs [PULL_FORALL]
+  \\ match_mp_tac (trans_app |> SIMP_RULE std_ss [LET_THM] |> MP_CANON |> GEN_ALL)
+  \\ fs [make_env_def]
+  \\ simp [read_str_code_def]
+  \\ simp [Eval_eq,PULL_EXISTS]
+  \\ fs [combinTheory.APPLY_UPDATE_THM,name_def]
+  \\ Cases_on ‘input’ \\ fs [next_def]
+  \\ fs [take_branch_def,return_def,Eval_eq,PULL_EXISTS,next_def,
+         combinTheory.APPLY_UPDATE_THM,eval_op_def,read_num_def]
+  \\ rpt BasicProvers.VAR_EQ_TAC
+  \\ fs [take_branch_def,return_def,Eval_eq,PULL_EXISTS,next_def,
+         combinTheory.APPLY_UPDATE_THM,eval_op_def,read_num_def]
+  THEN1 fs [state_component_equality]
+  \\ reverse IF_CASES_TAC
+  \\ fs [take_branch_def,return_def,Eval_eq,PULL_EXISTS,next_def,
+         combinTheory.APPLY_UPDATE_THM,eval_op_def,read_num_def]
+  THEN1 (rw [] \\ fs [state_component_equality,next_def])
+  \\ fs [take_branch_def,return_def,Eval_eq,PULL_EXISTS,next_def,
+         combinTheory.APPLY_UPDATE_THM,eval_op_def,read_num_def]
+  \\ IF_CASES_TAC
+  \\ fs [take_branch_def,return_def,Eval_eq,PULL_EXISTS,next_def,
+         combinTheory.APPLY_UPDATE_THM,eval_op_def,read_num_def]
+  THEN1 (rw [] \\ fs [state_component_equality,next_def])
+  \\ (theorem "mul256_app" |> DISCH_ALL |> Q.INST [‘n’|->‘acc’]
+         |> SIMP_RULE (srw_ss()) [] |> mp_tac)
+  \\ fs [name_def,llistTheory.LFINITE_fromList]
+  \\ strip_tac \\ goal_assum (first_assum o mp_then Any mp_tac)
+  \\ fs [] \\ Cases_on ‘t’ \\ fs [AND_IMP_INTRO]
+  \\ first_x_assum (first_assum o mp_then (Pos (el 2)) mp_tac)
+  \\ fs []
+  THEN1 (disch_then (qspec_then ‘s with input := fromList ""’ mp_tac) \\ fs [])
+  \\ disch_then (qspec_then ‘s with input := fromList t'’ mp_tac) \\ fs []
+QED
+
+val end_line_code_def = define_code ‘
+  (defun end_line (next)
+     (if (< next '256)
+       (if (= next '10) (read) (end_line (read)))
+       next))’
+
+Theorem end_line_thm:
+  ∀input s.
+    lookup_fun (name "end_line") s.funs = SOME ([name "next"],end_line_code) ∧
+    s.input = fromList (TL input) ⇒
+    app (name "end_line") [next (fromList input)] s
+      (next (fromList (end_line input)), s with input := fromList (TL (end_line input)))
+Proof
+  simp [] \\ gen_tac \\ completeInduct_on ‘LENGTH input’
+  \\ rpt strip_tac \\ fs [PULL_FORALL]
+  \\ match_mp_tac (trans_app |> SIMP_RULE std_ss [LET_THM] |> MP_CANON |> GEN_ALL)
+  \\ fs [make_env_def]
+  \\ simp [end_line_code_def]
+  \\ simp [Eval_eq,PULL_EXISTS]
+  \\ fs [combinTheory.APPLY_UPDATE_THM,name_def]
+  \\ Cases_on ‘input’ \\ fs [next_def]
+  \\ fs [take_branch_def,return_def,Eval_eq,PULL_EXISTS,next_def,
+         combinTheory.APPLY_UPDATE_THM,eval_op_def,read_num_def]
+  THEN1 fs [state_component_equality,lex_def,end_line_def,next_def]
+  \\ fs [ORD_BOUND]
+  \\ fs [take_branch_def,return_def,Eval_eq,PULL_EXISTS,next_def,
+         combinTheory.APPLY_UPDATE_THM,eval_op_def,read_num_def]
+  \\ fs [end_line_def]
+  \\ Cases_on ‘h’ \\ fs []
+  \\ IF_CASES_TAC \\ fs []
+  \\ simp [Eval_eq,PULL_EXISTS]
+  \\ fs [take_branch_def,return_def,Eval_eq,PULL_EXISTS,next_def,
+         combinTheory.APPLY_UPDATE_THM,eval_op_def,read_num_def]
+  \\ fs [AND_IMP_INTRO,state_component_equality]
+  THEN1 (Cases_on ‘t’ \\ fs [])
+  \\ first_x_assum (qspecl_then [‘t’,‘s with input := fromList (TL t)’] mp_tac) \\ fs []
+  \\ Cases_on ‘t’ \\ fs []
+QED
+
+val lex_code_def = define_code ‘
+  (defun lex (q next acc)
+     (if (< next '* )
+       (let (n (read))
+         (if (= next '40) (lex '0 n (cons (OPEN) acc))
+           (if (= next '41) (lex '0 n (cons (CLOSE) acc))
+             (if (= next '39) (lex '1 n acc)
+               (if (= next '35) (lex '0 (end_line n) acc)
+                 (lex '0 n acc))))))
+       (if (= next '46)
+         (lex '0 (read) (cons (DOT) acc))
+         (if (< 'z next)
+           (if (< next '256)
+             (lex '0 (read) acc) acc)
+             (let (r (read_any next))
+               (lex '0 (tail r)
+                 (if (= q '0)
+                   (cons (NUM (head r)) acc)
+                   (cons (QUOTE (head r)) acc))))))))’
+
+val lexer_code_def = define_code ‘
+  (defun lexer ()
+     (lex '0 (read) '0))’
+
+Triviality LTL_fromList_lemma[simp]:
+  (case LTL (fromList t) of NONE => fromList t | SOME t => t) = fromList (TL t)
+Proof
+  Cases_on ‘t’ \\ fs []
+QED
+
+Theorem lex_thm:
+  ∀input s acc k toks.
+    lookup_fun (name "mul10") s.funs = SOME ([name "n"],mul10_code) ∧
+    lookup_fun (name "mul256") s.funs = SOME ([name "n"],mul256_code) ∧
+    lookup_fun (name "end_line") s.funs = SOME ([name "next"],end_line_code) ∧
+    lookup_fun (name "read_num") s.funs = SOME ([name "acc"; name "next"],read_num_code) ∧
+    lookup_fun (name "read_str") s.funs = SOME ([name "acc"; name "next"],read_str_code) ∧
+    lookup_fun (name "read_any") s.funs = SOME ([name "next"],read_any_code) ∧
+    lookup_fun (name "lex") s.funs = SOME ([name "q"; name "next"; name "acc"],lex_code) ∧
+    s.input = fromList (TL input) ∧
+    lex (if k = 0 then NUM else QUOTE) input acc = toks ⇒
+    app (name "lex") [Num k; next (fromList input); list token acc] s
+      (list token toks, s with input := fromList [])
+Proof
+  simp [] \\ gen_tac \\ completeInduct_on ‘LENGTH input’
+  \\ rw [] \\ fs [PULL_FORALL]
+  \\ match_mp_tac (trans_app |> SIMP_RULE std_ss [LET_THM] |> MP_CANON |> GEN_ALL)
+  \\ fs [make_env_def]
+  \\ simp_tac std_ss [Once lex_code_def]
+  \\ simp_tac (srw_ss()) [Once Eval_eq,PULL_EXISTS]
+  \\ fs [combinTheory.APPLY_UPDATE_THM,name_def]
+  \\ Cases_on ‘input’ \\ fs [next_def]
+  \\ fs [take_branch_def,return_def,Eval_eq,PULL_EXISTS,next_def,
+         combinTheory.APPLY_UPDATE_THM,eval_op_def,read_num_def]
+  THEN1 fs [state_component_equality,lex_def]
+  \\ IF_CASES_TAC
+  \\ rpt BasicProvers.var_eq_tac
+  \\ fs [take_branch_def,return_def,Eval_eq,PULL_EXISTS,next_def,
+         combinTheory.APPLY_UPDATE_THM,eval_op_def,read_num_def]
+  THEN1
+   (IF_CASES_TAC
+    \\ fs [Eval_eq,PULL_EXISTS,combinTheory.APPLY_UPDATE_THM,eval_op_def,return_def]
+    THEN1
+     (Cases_on ‘h’ \\ fs [lex_def] \\ rw [] \\ fs [AND_IMP_INTRO]
+      \\ first_x_assum (qspecl_then [‘t’,
+           ‘s with input := fromList (TL t)’,‘OPEN::acc’,‘0’] mp_tac)
+      \\ fs [name_def])
+    \\ fs [Eval_eq,eval_op_def,return_def, take_branch_def]
+    \\ IF_CASES_TAC
+    THEN1
+     (Cases_on ‘h’ \\ fs [lex_def] \\ rw []
+      \\ fs [AND_IMP_INTRO,PULL_EXISTS,Eval_eq,combinTheory.APPLY_UPDATE_THM,
+             eval_op_def,return_def]
+      \\ first_x_assum (qspecl_then [‘t’,
+           ‘s with input := fromList (TL t)’,‘CLOSE::acc’,‘0’] mp_tac)
+      \\ fs [name_def])
+    \\ fs [Eval_eq,eval_op_def,return_def, take_branch_def,PULL_EXISTS,
+           combinTheory.APPLY_UPDATE_THM]
+    \\ IF_CASES_TAC
+    THEN1
+     (Cases_on ‘h’ \\ fs [lex_def] \\ rw []
+      \\ fs [AND_IMP_INTRO,PULL_EXISTS,Eval_eq,combinTheory.APPLY_UPDATE_THM,
+             eval_op_def,return_def]
+      \\ first_x_assum (qspecl_then [‘t’,
+           ‘s with input := fromList (TL t)’,‘acc’,‘1’] mp_tac)
+      \\ fs [name_def])
+    \\ fs [Eval_eq,eval_op_def,return_def, take_branch_def,PULL_EXISTS,
+           combinTheory.APPLY_UPDATE_THM]
+    \\ IF_CASES_TAC
+    THEN1
+     (Cases_on ‘h’ \\ fs [lex_def] \\ rw []
+      \\ fs [AND_IMP_INTRO,PULL_EXISTS,Eval_eq,combinTheory.APPLY_UPDATE_THM,
+             eval_op_def,return_def]
+      \\ qspecl_then [‘t’,‘s with input := fromList (TL t)’] mp_tac
+           (SIMP_RULE (srw_ss()) [name_def] end_line_thm)
+      \\ fs [next_def]
+      \\ strip_tac \\ goal_assum (first_assum o mp_then Any mp_tac)
+      \\ first_x_assum (qspecl_then [‘end_line t’,
+            ‘s with input := fromList (TL (end_line t))’,‘acc’,‘0’] mp_tac)
+      \\ fs [name_def]
+      \\ disch_then match_mp_tac \\ fs [end_line_length])
+    \\ fs [Eval_eq,eval_op_def,return_def, take_branch_def,PULL_EXISTS,
+           combinTheory.APPLY_UPDATE_THM]
+    \\ Cases_on ‘h’ \\ fs [lex_def] \\ rw [] \\ fs []
+    \\ first_x_assum (qspecl_then [‘t’,‘s with input := fromList (TL t)’,‘acc’,‘0’]
+                      mp_tac) \\ fs [name_def]
+    \\ fs [read_num_def])
+  \\ IF_CASES_TAC
+  THEN1
+   (Cases_on ‘h’ \\ fs [lex_def] \\ rw []
+    \\ fs [AND_IMP_INTRO,PULL_EXISTS,Eval_eq,combinTheory.APPLY_UPDATE_THM,
+           eval_op_def,return_def]
+    \\ first_x_assum (qspecl_then [‘t’,‘s with input := fromList (TL t)’,‘DOT::acc’,‘0’]
+                      mp_tac) \\ fs [name_def,next_def])
+  \\ fs [AND_IMP_INTRO,PULL_EXISTS,Eval_eq,combinTheory.APPLY_UPDATE_THM,
+         eval_op_def,return_def,take_branch_def]
+  \\ IF_CASES_TAC
+  THEN1
+   (fs [AND_IMP_INTRO,PULL_EXISTS,Eval_eq,combinTheory.APPLY_UPDATE_THM,
+        eval_op_def,return_def,take_branch_def,ORD_BOUND]
+    \\ first_x_assum (qspecl_then [‘t’,‘s with input := fromList (TL t)’,‘acc’,‘0’]
+                      mp_tac) \\ fs [name_def,lex_def]
+    \\ rw [] \\ fs [read_num_def,next_def])
+  \\ fs [AND_IMP_INTRO,PULL_EXISTS,Eval_eq,combinTheory.APPLY_UPDATE_THM,
+         eval_op_def,return_def,take_branch_def,ORD_BOUND]
+  \\ fs [lex_def]
+  \\ qpat_abbrev_tac ‘pp2 = if k = 0 then _ else _’
+  \\ qpat_abbrev_tac ‘pp = if k = 0 then _ else _’
+  \\ rw [] \\ fs []
+  \\ simp [Once app_cases,PULL_EXISTS,env_and_body_def,make_env_def]
+  \\ fs [AND_IMP_INTRO,PULL_EXISTS,Eval_eq,combinTheory.APPLY_UPDATE_THM,name_def,
+         eval_op_def,return_def,take_branch_def,read_any_code_def]
+  \\ reverse (Cases_on ‘ORD #"0" ≤ ORD h ⇒ ORD #"9" < ORD h’) \\ fs [NOT_LESS]
+  THEN1
+   (fs [AND_IMP_INTRO,PULL_EXISTS,Eval_eq,combinTheory.APPLY_UPDATE_THM,name_def,
+        eval_op_def,return_def,take_branch_def,read_any_code_def]
+    \\ pairarg_tac \\ fs []
+    \\ drule (read_num_thm |> SIMP_RULE (srw_ss()) []) \\ fs [next_def]
+    \\ disch_then (qspec_then ‘s’ mp_tac) \\ fs [name_def]
+    \\ strip_tac \\ goal_assum (first_assum o mp_then Any mp_tac)
+    \\ fs [] \\ reverse IF_CASES_TAC
+    THEN1
+     (fs [] \\ rfs [read_num_def]
+      \\ imp_res_tac read_num_length \\ fs [])
+    \\ unabbrev_all_tac \\ fs []
+    \\ Cases_on ‘k = 0’ \\ fs []
+    \\ fs [PULL_EXISTS,Eval_eq,combinTheory.APPLY_UPDATE_THM,name_def,
+           eval_op_def,return_def,take_branch_def]
+    \\ imp_res_tac read_num_length \\ fs []
+    \\ first_x_assum (qspecl_then [‘rest’,‘s with input := fromList (TL rest)’,
+         ‘if k = 0 then NUM n::acc else QUOTE n::acc’,‘0’] mp_tac)
+    \\ fs [name_def])
+  \\ fs [AND_IMP_INTRO,PULL_EXISTS,Eval_eq,combinTheory.APPLY_UPDATE_THM,
+         eval_op_def,return_def,take_branch_def,read_any_code_def,name_def]
+  \\ IF_CASES_TAC
+  \\ pairarg_tac \\ fs []
+  \\ pop_assum (mp_tac o REWRITE_RULE [read_num_def]) \\ fs []
+  \\ rw []
+  \\ fs [AND_IMP_INTRO,PULL_EXISTS,Eval_eq,combinTheory.APPLY_UPDATE_THM,
+         eval_op_def,return_def,take_branch_def,name_def]
+  \\ pairarg_tac \\ fs []
+  \\ drule (read_str_thm |> SIMP_RULE (srw_ss()) []) \\ fs [next_def,name_def]
+  \\ disch_then (qspec_then ‘s’ mp_tac) \\ fs [name_def]
+  \\ strip_tac \\ goal_assum (first_assum o mp_then Any mp_tac)
+  \\ fs [] \\ (reverse IF_CASES_TAC
+  THEN1 (fs [] \\ rfs [read_num_def] \\ imp_res_tac read_num_length \\ fs []))
+  \\ ‘rest' ≠ STRING h t’ by fs [read_num_def]
+  \\ unabbrev_all_tac \\ fs []
+  \\ Cases_on ‘k = 0’ \\ fs []
+  \\ fs [PULL_EXISTS,Eval_eq,combinTheory.APPLY_UPDATE_THM,name_def,
+         eval_op_def,return_def,take_branch_def]
+  \\ imp_res_tac read_num_length \\ fs []
+  \\ first_x_assum (qspecl_then [‘rest'’,
+       ‘s with input := fromList (TL rest')’,
+       ‘if k = 0 then NUM n' :: acc else QUOTE n'::acc’,‘0’] mp_tac)
+  \\ fs [name_def] \\ rfs []
+QED
+
+Theorem lexer_thm:
+  lookup_fun (name "mul10") s.funs = SOME ([name "n"],mul10_code) ∧
+  lookup_fun (name "mul256") s.funs = SOME ([name "n"],mul256_code) ∧
+  lookup_fun (name "end_line") s.funs = SOME ([name "next"],end_line_code) ∧
+  lookup_fun (name "read_num") s.funs = SOME ([name "acc"; name "next"],read_num_code) ∧
+  lookup_fun (name "read_str") s.funs = SOME ([name "acc"; name "next"],read_str_code) ∧
+  lookup_fun (name "read_any") s.funs = SOME ([name "next"],read_any_code) ∧
+  lookup_fun (name "lex") s.funs = SOME ([name "q"; name "next"; name "acc"],lex_code) ∧
+  lookup_fun (name "lexer") s.funs = SOME ([],lexer_code) ∧
+  s.input = fromList input ⇒
+  app (name "lexer") [] s (list token (lexer input), s with input := LNIL)
+Proof
+  rw []
+  \\ match_mp_tac (trans_app |> SIMP_RULE std_ss [LET_THM] |> MP_CANON |> GEN_ALL)
+  \\ fs [make_env_def]
+  \\ simp [lexer_code_def]
+  \\ simp [Eval_eq,PULL_EXISTS,eval_op_def,return_def]
+  \\ qspecl_then [‘input’,‘s with input := fromList (TL input)’,‘[]’,‘0’]
+       mp_tac (lex_thm |> SIMP_RULE std_ss [])
+  \\ fs [lexer_def]
+QED
+
+(* asm2str *)
+
+val res = to_deep x64asm_syntaxTheory.reg_def;
+
+Theorem num_thm: (* this rephrasing avoids MOD, which is not supported *)
+  num n s =
+    if n < 10 then (CHR (48 + n))::s else
+      let d = n DIV 10 in
+      let m = n - mul10 d in
+        num d ((CHR (48 + m)) :: s)
+Proof
+  simp [Once x64asm_syntaxTheory.num_def]
+  \\ rw [] \\ ‘0 < 10n’ by fs []
+  \\ drule DIVISION
+  \\ disch_then (qspec_then ‘n’ strip_assume_tac)
+  \\ AP_TERM_TAC \\ AP_THM_TAC \\ rpt AP_TERM_TAC \\ decide_tac
+QED
+
+Definition num_temp:
+  num_temp n s =
+    if n < 10 then (CHR (48 + n))::s else
+      let d = n DIV 10 in
+      let m = n - mul10 d in
+        num_temp d ((CHR (48 + m)) :: s)
+End
+
+Theorem num_ind = num_temp_ind
+
+val res = to_deep num_thm
+
+Triviality num_side:
+  ∀n s. num_side n s ⇔ T
+Proof
+  completeInduct_on ‘n’ \\ fs []
+  \\ once_rewrite_tac [res]
+  \\ Cases_on ‘n < 10’ \\ fs []
+  \\ rw [] \\ ‘0 < 10n’ by fs []
+  \\ drule DIVISION
+  \\ disch_then (qspec_then ‘n’ strip_assume_tac)
+  \\ decide_tac
+QED
+
+val _ = update_mem num_side;
+
+val res = to_deep lab_def
+val res = to_deep x64asm_syntaxTheory.clean_def
+
+Definition mul8_def:
+  mul8 n =
+    let n = n + n in
+    let n = n + n in
+      n + n : num
+End
+
+val res = to_deep mul8_def;
+
+Theorem mul8_thm[simp]:
+  mul8_side n = T ∧
+  mul8 n = 8 * n
+Proof
+  fs [mul8_def,res]
+QED
+
+val res = to_deep (x64asm_syntaxTheory.inst_def |> REWRITE_RULE [GSYM mul8_thm])
+val res = to_deep x64asm_syntaxTheory.insts_def
+val lemma = asm2str_def |> concl |> find_term (can (match_term “FLAT _”)) |> EVAL
+val res = to_deep (asm2str_def |> SIMP_RULE std_ss [lemma])
+
+(* print *)
+
+val print_code_def = define_code ‘
+  (defun print (s)
+     (if (= s '0) '0
+       (let
+         (a (write (head s)))
+         (print (tail s)))))’
+
+Theorem print_thm:
+  ∀str s.
+    lookup_fun (name "print") s.funs = SOME ([name "s"],print_code) ⇒
+    app (name "print") [list char str] s
+      (Num 0, s with output := s.output ++ str)
+Proof
+  gen_tac \\ completeInduct_on ‘LENGTH str’
+  \\ rw [] \\ fs [PULL_FORALL]
+  \\ match_mp_tac (trans_app |> SIMP_RULE std_ss [LET_THM] |> MP_CANON |> GEN_ALL)
+  \\ fs [make_env_def]
+  \\ simp [print_code_def]
+  \\ simp [Eval_eq,PULL_EXISTS]
+  \\ fs [combinTheory.APPLY_UPDATE_THM]
+  \\ rename [‘list (MAP char t)’]
+  \\ Cases_on ‘t’ \\ fs []
+  \\ fs [list_def,take_branch_def,return_def]
+  \\ simp [Eval_eq,PULL_EXISTS]
+  THEN1 fs [state_component_equality]
+  \\ fs [combinTheory.APPLY_UPDATE_THM,eval_op_def,return_def,ORD_BOUND]
+  \\ fs [name_def,AND_IMP_INTRO,CHR_ORD]
+  \\ first_x_assum (qspecl_then [‘t'’,
+      ‘s with output := STRCAT s.output (STRING h "")’] mp_tac)
+  \\ fs [] \\ simp_tac std_ss [GSYM APPEND_ASSOC,APPEND]
+QED
+
+(* definition of whole program *)
+
+local
+val _ = max_print_depth := 15;
+val main_exp = parse_exp ‘(print (asm2str (codegen (parser (lexer)))))’;
+val entire_program = get_program main_exp;
+in
 
 Definition compiler_prog_def:
-  compiler_prog = Program [] ARB : source_syntax$prog
+  compiler_prog = ^entire_program :source_syntax$prog
 End
+
+Theorem compiler_prog_thm[local] =
+        compiler_prog_def |> CONV_RULE (RAND_CONV EVAL);
+
+Definition coms_def:
+  coms = ^(get_comments ())
+End
+
+end
+
+(* proving that it's correct *)
+
+Theorem compiler_prog_correct:
+  ∀input. (input, compiler_prog) prog_terminates (imp_compiler$compiler input)
+Proof
+  rw [source_semanticsTheory.prog_terminates_def,compiler_prog_thm,compiler_def]
+  \\ qpat_abbrev_tac ‘pat = Defun _ _ _ :: _’
+  \\ simp [Eval_eq,PULL_EXISTS]
+  \\ qspecl_then [‘init_state (fromList input) pat’,‘input’]
+       mp_tac (GEN_ALL lexer_thm)
+  \\ impl_tac THEN1
+    (rewrite_tac [read_num_code_def,read_str_code_def,read_any_code_def,
+                  lex_code_def,lexer_code_def,end_line_code_def]
+     \\ rpt strip_tac \\ unabbrev_all_tac \\ EVAL_TAC)
+  \\ simp [name_def] \\ strip_tac
+  \\ goal_assum (first_x_assum o mp_then Any mp_tac)
+  \\ ‘init_state (fromList input) pat with input := LNIL = init_state LNIL pat’ by
+      simp [init_state_def]
+  \\ simp [] \\ pop_assum kall_tac
+  \\ ‘∀input. (init_state input pat).input = input’ by (EVAL_TAC \\ fs [])
+  \\ simp [] \\ pop_assum kall_tac
+  \\ irule_at Any (fetch "-" "parser_app" |> DISCH_ALL |> REWRITE_RULE [AND_IMP_INTRO]
+                                                       |> SRULE [name_def])
+  \\ simp [GSYM PULL_EXISTS] \\ rewrite_tac [CONJ_ASSOC]
+  \\ conj_tac
+  >- (unabbrev_all_tac \\ EVAL_TAC \\ fs [llistTheory.LFINITE_THM])
+  \\ irule_at Any (fetch "-" "codegen_app" |> DISCH_ALL |> REWRITE_RULE [AND_IMP_INTRO]
+                                                        |> SRULE [name_def])
+  \\ simp [GSYM PULL_EXISTS] \\ rewrite_tac [CONJ_ASSOC]
+  \\ conj_tac
+  >- (unabbrev_all_tac \\ EVAL_TAC \\ fs [llistTheory.LFINITE_THM])
+  \\ irule_at Any (fetch "-" "asm2str_app" |> DISCH_ALL |> REWRITE_RULE [AND_IMP_INTRO]
+                                                        |> SRULE [name_def])
+  \\ simp [GSYM PULL_EXISTS] \\ rewrite_tac [CONJ_ASSOC]
+  \\ conj_tac
+  >- (unabbrev_all_tac \\ EVAL_TAC \\ fs [llistTheory.LFINITE_THM])
+  \\ irule_at Any (print_thm |> DISCH_ALL |> REWRITE_RULE [AND_IMP_INTRO]
+                                          |> SRULE [name_def])
+  \\ simp [str2imp_def]
+  \\ unabbrev_all_tac \\ EVAL_TAC \\ simp [print_code_def] \\ EVAL_TAC
+QED
